MultiScalarMul_Abstract_Soundness.ec
@@ -14,52 +14,6 @@ declare module O <: OutCalls.
 
 declare axiom O_lossless : islossless O.getU. 
 
-lemma multieqs2 argP args argU  :
- equiv [ SimpleComp.multiScalarMulMain_Perfect 
-        ~ SimpleComp.multiScalarMulMain_Opt_Corrected :
-  arg{2} = (argP, args, argU) /\ ={P,s,U} /\ ={glob O}
-     ==>  res{2}.`1 => (res{1} = res{2}.`2)].
-proc.
-wp.
-inline SimpleComp.multiScalarMulMain_Opt.
-inline   SimpleComp.multiScalarMulMain_Perfect_Helper.
-       wp.
-while ((flag0{2} => ={table,acc,U,s} /\ (forall i j, table{2} i j <> idR)) /\ (flag0{2} => flagaux{2}) /\ ={ic} /\ s0{1} = s0{2}  ).
-wp.
-inline SimpleComp.completeAddLoop.
-inline SimpleComp.incompleteAddLoop.   
-wp.
-while ((flag0{2} /\ flag1{2} => ={vahe, acc0,table0,aux0,ic0} /\ (forall i j, table0{2} i j <> idR) /\ vahe{2} <> idR) /\ ={jc0} /\ s1{1} = s1{2} ).
- wp. skip. progress.
-   have -> : vahe{1} = vahe{2}. smt().
-rewrite same_res. 
-  smt().
-  smt().
-  smt().
-  smt().
-  smt().
-     smt().
-     smt().
-     smt().
-     smt().
-
-apply opt_never_id. smt(). smt().
-smt().
-wp.
-ecall {1} (doublewtimes_spec_ph acc{1} w).
-ecall {2} (doublewtimes_spec_ph acc{2} w).
-skip. progress. 
-smt(w_pos). smt(). smt(). smt().
-smt(). 
-apply no_order_two_elems. smt(w_pos). 
-smt(). smt(). smt().
-smt(). smt().     admit. admit.
-wp. 
- skip. progress. admit.
-smt().
-qed.
-
-
 
 
 lemma multiscalarI_spec_ph argP args  argU : 
@@ -70,21 +24,22 @@ proof.
 bypr.
 progress.
 have ih: 1%r = Pr[SimpleComp.multiScalarMulMain_Perfect(P{m}, s{m}, U{m}) @ &m 
-  : res = multiScalarMul_Simpl args argP T l].
+  : res.`2 = multiScalarMul_Simpl args argP T l].
 byphoare (_: arg = (argP, args, argU) ==> _).
 conseq (multiscalarR_spec_ph argP args argU). smt(). auto.
 have : Pr[SimpleComp.multiScalarMulMain_Opt_Corrected(P{m}, s{m}, U{m}) @ &m :
    res.`1 => res.`2 = multiScalarMul_Simpl args argP T l] >=
 Pr[SimpleComp.multiScalarMulMain_Perfect(P{m}, s{m}, U{m}) @ &m :
-   res = multiScalarMul_Simpl args argP T l].
-byequiv (_: ={glob O} /\ arg{2} = (P{m}, s{m}, U{m}) /\ arg{1} = (P{m}, s{m}, U{m}) ==> res{2}.`1 => res{2}.`2 = res{1} ).
+   res.`2 = multiScalarMul_Simpl args argP T l].
+byequiv (_: ={glob O} /\ arg{2} = (P{m}, s{m}, U{m}) /\ arg{1} = (P{m}, s{m}, U{m}) ==> res{2}.`1 => res{2}.`2 = res.`2{1} ).
 proc*.
 ecall (multieqs2 argP args argU).
 skip. progress. smt(). smt(). smt(). 
 auto.
 smt().
 smt.
-auto.
+auto. 
+smt.
 smt.
 qed.
 
@@ -101,7 +56,7 @@ apply O_lossless.
  auto.   
 exists* u_cand. elim*. move => u_candV.
 call (multiscalarI_spec_ph  argP args u_candV).
-wp.   skip. progress. rewrite H. auto.
+wp.   skip. progress. 
 hoare. simplify. call(_:true). auto. auto.
  qed.   
 
